@prefix sbeo: <http://www.ia.urjc.es/ontologies/building/sbeo#> .
@prefix owl: <http://www.w3.org/2002/07/owl#> .
@prefix rdf: <http://www.w3.org/1999/02/22-rdf-syntax-ns#> .
@prefix xsd: <http://www.w3.org/2001/XMLSchema#> .
@prefix foaf: <http://xmlns.com/foaf/0.1/> .
@prefix rdfs: <http://www.w3.org/2000/01/rdf-schema#> .
@prefix seas: <https://w3id.org/seas/> .
@prefix saref: <https://w3id.org/saref#> .
@prefix terms: <http://purl.org/dc/terms/> .
@prefix dcterms: <http://purl.org/dc/terms/> .
@prefix fiemser: <http://sites.google.com/site/smartappliancesproject/ontologies/fiemser#> .
@base <http://www.ia.urjc.es/ontologies/building/sbeo> .

<http://www.ia.urjc.es/ontologies/building/sbeo> rdf:type owl:Ontology ;
                                                    owl:versionIRI <http://www.ia.urjc.es/ontologies/building/sbeo/1.7> ;
                                                    owl:imports seas:BuildingOntology-1.0 ;
                                                    dcterms:creator "Qasim Khalid" ;
                                                    dcterms:description "The Smart Buildings Evacuation Ontology (SBEO) is proposed to acquire knowledge of emergency evacuation (or egress) and to provide safe evacuation paths to the occupants of buildings during hazardous circumstances in a building. The goal of this ontology is not only to provide safe paths to the people, but also the paths will be feasible for people with respect to their physical characteristics and preferences. In this regard, we propose a knowledge base system for emergency evacuation in which we use the concept of a smart building. First, we define the concepts that are necessary to develop the proposed systems. Second, we develop the hierarchy to use these concepts. Third, we define the properties and characteristics of these concepts. Fourth, we introduce role restrictions, and at last, we introduce instances for particular scenarios to validate our foundation knowledge base. We use three different concepts in our ontology and integrate them with respect to our requirements. The first concept is knowledge about the building geometry, the second concept is the knowledge about the momentary situation of the building, and the third concept is the knowledge about the occupants of the building. We reuse seas:BuildingOntology to get geometry of the buildings. Also, it may limit the overlap with the following existing specialized ontologies such as FIEMSER ontology, gbXML ontology and ifcOWL ontology."^^xsd:string ;
                                                    dcterms:title "SBEO: Smart Building Evacuation Ontology" ;
                                                    owl:versionInfo 1.7 .

#################################################################
#    Object Properties
#################################################################

###  http://www.ia.urjc.es/ontologies/building/sbeo#accompanying
sbeo:accompanying rdf:type owl:ObjectProperty ,
                             owl:SymmetricProperty ,
                             owl:TransitiveProperty ;
                    rdfs:domain sbeo:Person ;
                    rdfs:range sbeo:Person ;
                    rdfs:comment "This property is used to mention how who is accompanying who."^^xsd:string ;
                    rdfs:label "accompanying"^^xsd:string .


###  http://www.ia.urjc.es/ontologies/building/sbeo#acquaintanceOf
sbeo:acquaintanceOf rdf:type owl:ObjectProperty ,
                               owl:SymmetricProperty ;
                      rdfs:domain sbeo:Person ;
                      rdfs:range sbeo:Person ;
                      rdfs:comment "This property is used to represent any friend or acquaintace tie among occupants."^^xsd:string ;
                      rdfs:label "acquaintanceOf"^^xsd:string .


###  http://www.ia.urjc.es/ontologies/building/sbeo#adjacentTo
sbeo:adjacentTo rdf:type owl:ObjectProperty ,
                           owl:SymmetricProperty ;
                  rdfs:domain seas:Zone ;
                  rdfs:range seas:Zone ;
                  rdfs:comment "This property is used to mention the spaces that are adjacent to a specific space by a wall. This property is helpful for security purposes, for example, in case of any emergency situation when the seas:BuildingSpaceConnection, i.e. door, windows, are not accessible."^^xsd:string ;
                  rdfs:label "adjacentTo"^^xsd:string .


###  http://www.ia.urjc.es/ontologies/building/sbeo#assignedRoute
sbeo:assignedRoute rdf:type owl:ObjectProperty ;
                     rdfs:subPropertyOf owl:topObjectProperty ;
                     rdfs:domain sbeo:Person ;
                     rdfs:range sbeo:Route ;
                     rdfs:comment "This property is used to represent a route (rdf:list of connected spaces) that is assigned to person for safe evacuation." ;
                     rdfs:label "assignedRoute" .


###  http://www.ia.urjc.es/ontologies/building/sbeo#connectedTo
sbeo:connectedTo rdf:type owl:ObjectProperty ;
                   owl:equivalentProperty seas:connectedTo ;
                   rdf:type owl:SymmetricProperty ;
                   rdfs:domain seas:BuildingSpace ,
                               seas:BuildingSpaceConnection ;
                   rdfs:range seas:BuildingSpace ,
                              seas:BuildingSpaceConnection ;
                   rdfs:comment "This property is used to mention the connectivity of any seas:BuildingSpaceConnection or seas:BuildingSpace with each other."^^xsd:string ;
                   rdfs:label "conectedTo"^^xsd:string .


###  http://www.ia.urjc.es/ontologies/building/sbeo#dependentOn
sbeo:dependentOn rdf:type owl:ObjectProperty ;
                   owl:inverseOf sbeo:responsibleTo ;
                   rdf:type owl:TransitiveProperty ;
                   rdfs:domain sbeo:Person ;
                   rdfs:range sbeo:Person ;
                   rdfs:comment "This property is used to mention the dependency of a particular person on his/her responsible person"^^xsd:string ;
                   rdfs:label "dependentOn"^^xsd:string .


###  http://www.ia.urjc.es/ontologies/building/sbeo#distanceOf
sbeo:distanceOf rdf:type owl:ObjectProperty ,
                           owl:SymmetricProperty ;
                  rdfs:domain sbeo:Distance ;
                  rdfs:range seas:Zone ,
                             seas:ZoneConnection ;
                  rdfs:comment "This property is used to represent the distance between any two connected seas:BuildingSpaceConnection or seas:BuildingSpace."^^xsd:string ;
                  rdfs:label "distanceOf"^^xsd:string .


###  http://www.ia.urjc.es/ontologies/building/sbeo#endsIn
sbeo:endsIn rdf:type owl:ObjectProperty ;
              owl:inverseOf sbeo:startsFrom ;
              rdfs:domain sbeo:Route ;
              rdfs:range seas:BuildingSpace ,
                         seas:BuildingSpaceConnection ;
              rdfs:comment "This property is used to express the last space where the route ends. Generally, these are sbeo:Exit."^^xsd:string ;
              rdfs:label "endsIn"^^xsd:string .


###  http://www.ia.urjc.es/ontologies/building/sbeo#hasPath
sbeo:hasPath rdf:type owl:ObjectProperty ;
               rdfs:domain seas:BuildingSpace ,
                           seas:BuildingSpaceConnection ;
               rdfs:range seas:BuildingSpace ,
                          seas:BuildingSpaceConnection ;
               rdfs:comment "This property is used to express the set of connected spaces that makes a route."^^xsd:string ;
               rdfs:label "hasPath"^^xsd:string .


###  http://www.ia.urjc.es/ontologies/building/sbeo#installedIn
sbeo:installedIn rdf:type owl:ObjectProperty ,
                            owl:TransitiveProperty ;
                   rdfs:domain sbeo:Device ,
                               seas:BuildingSpace ,
                               seas:BuildingSpaceConnection ;
                   rdfs:range seas:BuildingSpace ,
                              seas:BuildingSpaceConnection ;
                   rdfs:comment "This property is used to mention any device, system, or instrument, installed in a seas:BuildingSpace."^^xsd:string ;
                   rdfs:label "installedIn"^^xsd:string .


###  http://www.ia.urjc.es/ontologies/building/sbeo#locatedIn
sbeo:locatedIn rdf:type owl:ObjectProperty ;
                 rdfs:subPropertyOf owl:topObjectProperty ;
                 rdf:type owl:TransitiveProperty ;
                 rdfs:domain sbeo:Incident ,
                             sbeo:Person ,
                             seas:Zone ,
                             seas:ZoneConnection ;
                 rdfs:range seas:BuildingSpaceConnection ,
                            seas:Zone ;
                 rdfs:comment "This property is used to mention the existence of anything in a particular seas:BuildingSpace, such as person, or stairs, doors, etc."^^xsd:string ;
                 rdfs:label "locatedIn"^^xsd:string .


###  http://www.ia.urjc.es/ontologies/building/sbeo#notAccessibleTo
sbeo:notAccessibleTo rdf:type owl:ObjectProperty ;
                       rdfs:domain seas:Zone ,
                                   seas:ZoneConnection ;
                       rdfs:range sbeo:Person ;
                       rdfs:comment "This property is used to prohibit the access of any specific person to a specific seas:BuildingSpace."^^xsd:string ;
                       rdfs:label "notAccessibleTo"^^xsd:string .


###  http://www.ia.urjc.es/ontologies/building/sbeo#responsibleTo
sbeo:responsibleTo rdf:type owl:ObjectProperty ;
                     rdfs:domain sbeo:Person ;
                     rdfs:range sbeo:Person ;
                     rdfs:comment "This property is used to mention the responsibility for a particular person to his/her dependent persons."^^xsd:string ;
                     rdfs:label "responsibleTo"^^xsd:string .


###  http://www.ia.urjc.es/ontologies/building/sbeo#startsFrom
sbeo:startsFrom rdf:type owl:ObjectProperty ;
                  rdfs:domain sbeo:Route ;
                  rdfs:range seas:Zone ,
                             seas:ZoneConnection ;
                  rdfs:comment "This property is used to express the last space where any route starts."^^xsd:string ;
                  rdfs:label "startsFrom"^^xsd:string .


#################################################################
#    Data properties
#################################################################

###  http://www.ia.urjc.es/ontologies/building/sbeo#accommodationCapacity
sbeo:accommodationCapacity rdf:type owl:DatatypeProperty ;
                             rdfs:domain seas:Zone ,
                                         seas:ZoneConnection ;
                             rdfs:range xsd:integer ;
                             rdfs:comment "This property is used to represent the accommodating capacity (in terms of persons) of a particular space."^^xsd:string ;
                             rdfs:label "accommodationCapacity"^^xsd:string .


###  http://www.ia.urjc.es/ontologies/building/sbeo#age
sbeo:age rdf:type owl:DatatypeProperty ;
           owl:equivalentProperty foaf:age ;
           rdfs:domain sbeo:Person ;
           rdfs:range xsd:integer ;
           rdfs:comment "The age of the person."^^xsd:string ;
           rdfs:label "age"^^xsd:string .


###  http://www.ia.urjc.es/ontologies/building/sbeo#atTime
sbeo:atTime rdf:type owl:DatatypeProperty ;
              rdfs:domain sbeo:EvacuationStatus ,
                          sbeo:Incident ,
                          sbeo:Person ,
                          sbeo:Sensor ;
              rdfs:range xsd:long ;
              rdfs:comment "This property is used to attach a timestamp with any particular event."^^xsd:string ;
              rdfs:label "atTime"^^xsd:string .


###  http://www.ia.urjc.es/ontologies/building/sbeo#currentOccupancy
sbeo:currentOccupancy rdf:type owl:DatatypeProperty ;
                        rdfs:domain seas:Zone ,
                                    seas:ZoneConnection ;
                        rdfs:range xsd:integer ;
                        rdfs:comment "This property is used to represent the current occupancy(in terms of persons) of a particular space."^^xsd:string ;
                        rdfs:label "currentOccupancy"^^xsd:string .


###  http://www.ia.urjc.es/ontologies/building/sbeo#familiarityWithBuilding
sbeo:familiarityWithBuilding rdf:type owl:DatatypeProperty ;
                               rdfs:domain sbeo:Person ;
                               rdfs:range xsd:boolean ;
                               rdfs:comment "This property is used to represent the familiarity of person with the building geometry."^^xsd:string ;
                               rdfs:label "familiarityWithBuilding"^^xsd:string .


###  http://www.ia.urjc.es/ontologies/building/sbeo#familyID
sbeo:familyID rdf:type owl:DatatypeProperty ;
                rdfs:domain sbeo:Person ;
                rdfs:range xsd:integer ;
                rdfs:comment "This property is used to represent an identity number(ID) of each family. All the members of a family have common ID."^^xsd:string ;
                rdfs:label "familyID"^^xsd:string .


###  http://www.ia.urjc.es/ontologies/building/sbeo#firstName
sbeo:firstName rdf:type owl:DatatypeProperty ;
                 rdfs:subPropertyOf owl:topDataProperty ;
                 rdfs:domain sbeo:Person ;
                 rdfs:range xsd:string ;
                 rdfs:comment "The first name of the person."^^xsd:string ;
                 rdfs:label "firstName"^^xsd:string .


###  http://www.ia.urjc.es/ontologies/building/sbeo#fitnessLevel
sbeo:fitnessLevel rdf:type owl:DatatypeProperty ;
                    rdfs:domain sbeo:Person ;
                    rdfs:range xsd:integer ;
                    rdfs:comment "This property is used to represent the fitness level of a person. For example, there are 5 levels. Upper three levels are appropriate and considered as safe whereas the below two levels are considered as dangerous and a particular person needs assistance. The person is considered as sbeo:Injured, if the levels are changed from upper three to lower two."^^xsd:string ;
                    rdfs:label "fitnessLevel"^^xsd:string .


###  http://www.ia.urjc.es/ontologies/building/sbeo#groupID
sbeo:groupID rdf:type owl:DatatypeProperty ;
               rdfs:domain sbeo:Person ;
               rdfs:range xsd:integer ;
               rdfs:comment "This property is used to represent an identity number(ID) that is assigned to people who are evacuating together and having the same sbeo:assignedRoute."^^xsd:string ;
               rdfs:label "groupID"^^xsd:string .


###  http://www.ia.urjc.es/ontologies/building/sbeo#hasID
sbeo:hasID rdf:type owl:DatatypeProperty ;
             rdfs:domain sbeo:Person ;
             rdfs:range xsd:integer ;
             rdfs:comment "This property is used to represent an identification number, which is unique for every occupant of the building. It is different than group and family ID. This ID number is used to calculate all the functionalities for a specific person, e.g. location, characteristics, preferences, etc."^^xsd:string ;
             rdfs:label "hasID"^^xsd:string .


###  http://www.ia.urjc.es/ontologies/building/sbeo#hasLength
sbeo:hasLength rdf:type owl:DatatypeProperty ;
                 rdfs:domain sbeo:Route ;
                 rdfs:range xsd:integer ;
                 rdfs:comment "This property is used to represent a value between any two building space connections. This value can be expressed in terms of time, distance, etc."^^xsd:string ;
                 rdfs:label "hasLength"^^xsd:string .


###  http://www.ia.urjc.es/ontologies/building/sbeo#lastName
sbeo:lastName rdf:type owl:DatatypeProperty ;
                owl:equivalentProperty foaf:lastName ;
                rdfs:subPropertyOf owl:topDataProperty ;
                rdfs:domain sbeo:Person ;
                rdfs:range xsd:string ;
                rdfs:comment "The last name of the person."^^xsd:string ;
                rdfs:label "lastName"^^xsd:string .


###  http://www.ia.urjc.es/ontologies/building/sbeo#name
sbeo:name rdf:type owl:DatatypeProperty ;
            owl:equivalentProperty foaf:name ;
            rdfs:domain sbeo:Exit ,
                        sbeo:Person ,
                        sbeo:Route ,
                        sbeo:SafeZone ,
                        seas:Zone ,
                        seas:ZoneConnection ,
                        seas:ZoneFrontier ;
            rdfs:range xsd:string ;
            rdfs:label "The name of the person, place or a thing."^^xsd:string ,
                       "name"^^xsd:string .


###  http://www.ia.urjc.es/ontologies/building/sbeo#needsSupervision
sbeo:needsSupervision rdf:type owl:DatatypeProperty ;
                        rdfs:domain sbeo:Person ;
                        rdfs:range xsd:boolean ;
                        rdfs:comment "This property is used to mention either a person needs a supervision or not."^^xsd:string ;
                        rdfs:label "needsSupervision"^^xsd:string .



#################################################################
#    Classes
#################################################################

###  http://www.ia.urjc.es/ontologies/building/sbeo#ActiveFireProtection
sbeo:ActiveFireProtection rdf:type owl:Class ;
                            rdfs:subClassOf sbeo:FireProtection ;
                            rdfs:comment "ActiveFireProtection"^^xsd:string ,
                                         "It is an integral part of the fire protection used as a first response to minimize the spread of fire and related effects."^^xsd:string .


###  http://www.ia.urjc.es/ontologies/building/sbeo#AssemblyPoint
sbeo:AssemblyPoint rdf:type owl:Class ;
                     rdfs:subClassOf sbeo:SafeZone ;
                     rdfs:comment "a place where people in an office, etc. should go if there is an emergency, for example, a fire (Cambridge English Dictionary) ."^^xsd:string ;
                     rdfs:label "AssemblyPoint"^^xsd:string .


###  http://www.ia.urjc.es/ontologies/building/sbeo#Available
sbeo:Available rdf:type owl:Class ;
                 owl:equivalentClass sbeo:SafeZone ;
                 rdfs:subClassOf sbeo:SpaceCharacteristic ;
                 owl:disjointWith sbeo:Unavailable ;
                 rdfs:comment "This is used to specify the availability of a parituclar space, route, etc. If its available, it means it can be accessible to sbeo:Person subject to the characteristics of that person."^^xsd:string ;
                 rdfs:label "Available"^^xsd:string .


###  http://www.ia.urjc.es/ontologies/building/sbeo#ChemicalSpill
sbeo:ChemicalSpill rdf:type owl:Class ;
                     rdfs:subClassOf sbeo:Incident ;
                     rdfs:comment "A hazardous event that happens due to the spillage or leakge of any toxic chemical in the building."^^xsd:string ;
                     rdfs:label "ChemicalSpill"^^xsd:string .


###  http://www.ia.urjc.es/ontologies/building/sbeo#Congestion
sbeo:Congestion rdf:type owl:Class ;
                  rdfs:subClassOf sbeo:Incident ;
                  rdfs:comment "An event that happens at bottlenecks when the flow of people increases than a provided limit due to herding (and similar phenomena of human behaviour), during an emergency evacuation process. As a result, overall escape time is increased."^^xsd:string ;
                  rdfs:label "Congestion"^^xsd:string .


###  http://www.ia.urjc.es/ontologies/building/sbeo#DayCare
sbeo:DayCare rdf:type owl:Class ;
               rdfs:subClassOf seas:Room ;
               rdfs:comment "A space for childcare supervised by a nanny while parents are at work."^^xsd:string ;
               rdfs:label "DayCare"^^xsd:string .


###  http://www.ia.urjc.es/ontologies/building/sbeo#Dependent
sbeo:Dependent rdf:type owl:Class ;
                 rdfs:subClassOf sbeo:PedestrianCharacteristic ;
                 owl:disjointWith sbeo:Responsible ;
                 rdfs:comment "It represents the dependency of a person on other persons in case of any emergency condition."^^xsd:string ;
                 rdfs:label "Dependent"^^xsd:string .


###  http://www.ia.urjc.es/ontologies/building/sbeo#Device
sbeo:Device rdf:type owl:Class ;
              rdfs:comment "A thing made or adapted for a particular purpose, especially a piece of mechanical or electronic equipment (Oxford Dictionary of English)."^^xsd:string ;
              rdfs:label "Device" .


###  http://www.ia.urjc.es/ontologies/building/sbeo#Distance
sbeo:Distance rdf:type owl:Class ;
                rdfs:subClassOf sbeo:SpaceCharacteristic ;
                rdfs:comment "Distance class is mainly used to mention the distance between two spaces(either connected or not). As the building is represented as a graph having nodes and egdes, where as edges represents the connection between two nodes, therefore, the weight of the edge is considered as the Distance. Later on, the Distance is used to calculate the evaucation routes."^^xsd:string ;
                rdfs:label "Distance"^^xsd:string .


###  http://www.ia.urjc.es/ontologies/building/sbeo#Earthquake
sbeo:Earthquake rdf:type owl:Class ;
                  rdfs:subClassOf sbeo:Incident ;
                  rdfs:comment "A sudden violent shaking of the ground, typically causing great destruction, as a result of movements within the earth's crust or volcanic action(Oxford Dictionary). It may cause a sudden panic among the occupants of the building."^^xsd:string ;
                  rdfs:label "Earthquake"^^xsd:string .


###  http://www.ia.urjc.es/ontologies/building/sbeo#EmergencyExit
sbeo:EmergencyExit rdf:type owl:Class ;
                     rdfs:subClassOf sbeo:Exit ;
                     rdfs:comment "Emerency exit is only used in case of any emergency conditions such fire, etc."^^xsd:string ;
                     rdfs:label "EmergencyExit"^^xsd:string .


###  http://www.ia.urjc.es/ontologies/building/sbeo#Entrance
sbeo:Entrance rdf:type owl:Class ;
                rdfs:subClassOf sbeo:SpaceCharacteristic ;
                rdfs:comment "Entrance represents a space or a door that is used to enter into a building. Normally, it is also used as an exit."^^xsd:string ;
                rdfs:label "Entrance"^^xsd:string .


###  http://www.ia.urjc.es/ontologies/building/sbeo#EvacuationStatus
sbeo:EvacuationStatus rdf:type owl:Class ;
                        rdfs:comment "The status of an evacuation process for each person."^^xsd:string ;
                        rdfs:label "EvacuationStatus"^^xsd:string .


###  http://www.ia.urjc.es/ontologies/building/sbeo#Exit
sbeo:Exit rdf:type owl:Class ;
            rdfs:subClassOf sbeo:SpaceCharacteristic ;
            rdfs:comment "Exit represents a space or a door that is used to exit the building. Generally, an exit is as same as an entrance."^^xsd:string ;
            rdfs:label "Exit"^^xsd:string .


###  http://www.ia.urjc.es/ontologies/building/sbeo#Family
sbeo:Family rdf:type owl:Class ;
              rdfs:subClassOf sbeo:PedestrianCharacteristic ;
              rdfs:comment "A group of persons having family ties between them."^^xsd:string ;
              rdfs:label "Family"^^xsd:string .


###  http://www.ia.urjc.es/ontologies/building/sbeo#Fire
sbeo:Fire rdf:type owl:Class ;
            rdfs:subClassOf sbeo:Incident ;
            rdfs:comment "An event that may burn different parts of the building and hazourdous for both the people and the building."^^xsd:string ;
            rdfs:label "Fire"^^xsd:string .


###  http://www.ia.urjc.es/ontologies/building/sbeo#FireDoor
sbeo:FireDoor rdf:type owl:Class ;
                rdfs:subClassOf sbeo:PassiveFireProtection ;
                rdfs:comment "A type of door used to minimize the spread of fire and related effects by isolating two connected spaces or sections in the building."^^xsd:string ;
                rdfs:label "FireDoor"^^xsd:string .


###  http://www.ia.urjc.es/ontologies/building/sbeo#FireExtinguisher
sbeo:FireExtinguisher rdf:type owl:Class ;
                        rdfs:subClassOf sbeo:ActiveFireProtection ;
                        rdfs:comment "An active fire protection instrument used by persons to blow out small scale fire."^^xsd:string ;
                        rdfs:label "FireExtinguisher"^^xsd:string .


###  http://www.ia.urjc.es/ontologies/building/sbeo#FireProtection
sbeo:FireProtection rdf:type owl:Class ;
                      rdfs:subClassOf sbeo:IncidentProtection ;
                      rdfs:comment "It is a practice to minimize the effects of potentially danger fires."^^xsd:string ;
                      rdfs:label "FireProtection"^^xsd:string .


###  http://www.ia.urjc.es/ontologies/building/sbeo#Hearing
sbeo:Hearing rdf:type owl:Class ;
               rdfs:subClassOf sbeo:SensoryImpairment ;
               rdfs:comment "It is a partial or total unability to hear. It is also known as Hearing loss."^^xsd:string ;
               rdfs:label "Hearing"^^xsd:string .


###  http://www.ia.urjc.es/ontologies/building/sbeo#Impaired
sbeo:Impaired rdf:type owl:Class ;
                owl:equivalentClass sbeo:Injured ;
                rdfs:subClassOf sbeo:PedestrianCharacteristic ;
                owl:disjointWith sbeo:Normal ;
                rdfs:comment "The state or fact of being impaired, especially in a specified faculty(Oxford Distionary of Language)."^^xsd:string ;
                rdfs:label "Impaired"^^xsd:string .


###  http://www.ia.urjc.es/ontologies/building/sbeo#InProgress
sbeo:InProgress rdf:type owl:Class ;
                  rdfs:subClassOf sbeo:NotSuccessful ;
                  rdfs:comment "It represents that the person is following the provided route and the evacuation process is in progress."^^xsd:string ;
                  rdfs:label "InProgress"^^xsd:string .


###  http://www.ia.urjc.es/ontologies/building/sbeo#Incident
sbeo:Incident rdf:type owl:Class ;
                rdfs:comment "An event or occurance that can be dangerous for the occupants of the building."^^xsd:string ;
                rdfs:label "Incident"^^xsd:string .


###  http://www.ia.urjc.es/ontologies/building/sbeo#IncidentProtection
sbeo:IncidentProtection rdf:type owl:Class ;
                          rdfs:subClassOf sbeo:Device ;
                          rdfs:comment "It is a practice to avoid and minimize the effects of potentially danger events for the occupants of the building as well as for the structure of building itself."^^xsd:string ;
                          rdfs:label "IncidentProtection"^^xsd:string .


###  http://www.ia.urjc.es/ontologies/building/sbeo#Injured
sbeo:Injured rdf:type owl:Class ;
               rdfs:subClassOf sbeo:PedestrianCharacteristic ;
               rdfs:comment "It represents an injury to a person during an evacuation process."^^xsd:string ;
               rdfs:label "Injured"^^xsd:string .


###  http://www.ia.urjc.es/ontologies/building/sbeo#KidsArea
sbeo:KidsArea rdf:type owl:Class ;
                rdfs:subClassOf seas:Room ;
                rdfs:comment "A space where children can play during the specific time while parents are either busy at work or doing different things such as shopping, seeing a doctor, etc. Normally, it is not supervised by anyone."^^xsd:string ;
                rdfs:label "KidsArea"^^xsd:string .


###  http://www.ia.urjc.es/ontologies/building/sbeo#LocationSensor
sbeo:LocationSensor rdf:type owl:Class ;
                      rdfs:subClassOf sbeo:Sensor ;
                      rdfs:comment "The location sensor is a part of indoor positioning system to detect the location of each person within the building."^^xsd:string ;
                      rdfs:label "LocationSensor"^^xsd:string .


###  http://www.ia.urjc.es/ontologies/building/sbeo#LowStamina
sbeo:LowStamina rdf:type owl:Class ;
                  rdfs:subClassOf sbeo:PhysicalImpairment ;
                  rdfs:comment "It is the unability to sustain physical or mental activity to a normal level."^^xsd:string ;
                  rdfs:label "LowStamina"^^xsd:string .


###  http://www.ia.urjc.es/ontologies/building/sbeo#Motorised
sbeo:Motorised rdf:type owl:Class ;
                 rdfs:subClassOf sbeo:Wheelchair ;
                 rdfs:comment "It is a kind of wheelchair that has either a mechanical engine or an electric battery. It has more speed than a traditional wheelchair."^^xsd:string ;
                 rdfs:label "Motorised"^^xsd:string .


###  http://www.ia.urjc.es/ontologies/building/sbeo#Non-Motorised
sbeo:Non-Motorised rdf:type owl:Class ;
                     rdfs:subClassOf sbeo:Wheelchair ;
                     rdfs:comment "A traditional wheelchair that is used by hands. It has significantly lower speed than motorised wheelchairs."^^xsd:string ;
                     rdfs:label "Non-Motorised"^^xsd:string .


###  http://www.ia.urjc.es/ontologies/building/sbeo#Normal
sbeo:Normal rdf:type owl:Class ;
              rdfs:subClassOf sbeo:PedestrianCharacteristic ;
              rdfs:comment "Persons who are not having any impairment."^^xsd:string ;
              rdfs:label "Normal"^^xsd:string .


###  http://www.ia.urjc.es/ontologies/building/sbeo#NormalExit
sbeo:NormalExit rdf:type owl:Class ;
                  rdfs:subClassOf sbeo:Exit ;
                  rdfs:comment "Normal exit is used to exit a building. It can be a door or the whole space in the building that is always considered safe."^^xsd:string ;
                  rdfs:label "NormalExit"^^xsd:string .


###  http://www.ia.urjc.es/ontologies/building/sbeo#NotSuccessful
sbeo:NotSuccessful rdf:type owl:Class ;
                     rdfs:subClassOf sbeo:EvacuationStatus ;
                     rdfs:comment "It represents that the evacuation is not completed by a person yet."^^xsd:string ;
                     rdfs:label "NotSuccessful"^^xsd:string .


###  http://www.ia.urjc.es/ontologies/building/sbeo#Obstructed
sbeo:Obstructed rdf:type owl:Class ;
                  rdfs:subClassOf sbeo:NotSuccessful ;
                  rdfs:comment "It represents that the person is obstrcuted during an evacuation process and not continuing one's evcuation."^^xsd:string ;
                  rdfs:label "Obstructed"^^xsd:string .


###  http://www.ia.urjc.es/ontologies/building/sbeo#Panic
sbeo:Panic rdf:type owl:Class ;
             rdfs:subClassOf sbeo:Incident ;
             rdfs:comment "A  sudden uncontrollable fear or anxiety, often causing wildly unthinking behaviour (Oxford Dictionary of English)."^^xsd:string ;
             rdfs:label "Panic"^^xsd:string .


###  http://www.ia.urjc.es/ontologies/building/sbeo#PassiveFireProtection
sbeo:PassiveFireProtection rdf:type owl:Class ;
                             rdfs:subClassOf sbeo:FireProtection ;
                             rdfs:comment "It is an integral component installed in the building while construction to resist the fire."^^xsd:string ;
                             rdfs:label "PassiveFireProtection"^^xsd:string .


###  http://www.ia.urjc.es/ontologies/building/sbeo#PedestrianCharacteristic
sbeo:PedestrianCharacteristic rdf:type owl:Class ;
                                rdfs:comment "PedestrianCharacteristic class defines features for each person that are helps system to find an appropriate route."^^xsd:string ;
                                rdfs:label "PedestrianCharacteristic"^^xsd:string .


###  http://www.ia.urjc.es/ontologies/building/sbeo#Person
sbeo:Person rdf:type owl:Class ;
              owl:equivalentClass foaf:Person ;
              rdfs:comment "It represents a single individual of any age and having any type of characteristics."^^xsd:string ;
              rdfs:label "Person"^^xsd:string .


###  http://www.ia.urjc.es/ontologies/building/sbeo#PhysicalImpairment
sbeo:PhysicalImpairment rdf:type owl:Class ;
                          rdfs:subClassOf sbeo:Impaired ;
                          rdfs:comment "A physical impairment is a condition in which any part of person's body is either  damaged or is not working properly."^^xsd:string ;
                          rdfs:label "PhysicalImpairment"^^xsd:string .


###  http://www.ia.urjc.es/ontologies/building/sbeo#Responsible
sbeo:Responsible rdf:type owl:Class ;
                   rdfs:subClassOf sbeo:PedestrianCharacteristic ;
                   rdfs:comment "This class represents either a person is reponsible to anyone or not. One may be reponsible to one/all of one's family members or any other person such as injured, impiared etc."^^xsd:string ;
                   rdfs:label "Responsible"^^xsd:string .


###  http://www.ia.urjc.es/ontologies/building/sbeo#Route
sbeo:Route rdf:type owl:Class ;
             rdfs:subClassOf sbeo:SpaceCharacteristic ;
             rdfs:comment "Route is a set of spaces connected to each other by a door that ultimately leads to any of the exits in the building. Technically, rdf:list is used to store it."^^xsd:string ;
             rdfs:label "Route"^^xsd:string .


###  http://www.ia.urjc.es/ontologies/building/sbeo#SafeZone
sbeo:SafeZone rdf:type owl:Class ;
                rdfs:subClassOf sbeo:SpaceCharacteristic ;
                rdfs:comment "A space that is considered safe during any type of incident in the building."^^xsd:string ;
                rdfs:label "SafeZone"^^xsd:string .


###  http://www.ia.urjc.es/ontologies/building/sbeo#Sensor
sbeo:Sensor rdf:type owl:Class ;
              owl:equivalentClass saref:Sensor ;
              rdfs:subClassOf sbeo:Device ;
              rdfs:comment "A sensor is device that detects or measures a physical property and records, indicates, or otherwise responds to it (Oxford Dictionary of English)."^^xsd:string ;
              rdfs:label "Sensor"^^xsd:string .


###  http://www.ia.urjc.es/ontologies/building/sbeo#SensoryImpairment
sbeo:SensoryImpairment rdf:type owl:Class ;
                         rdfs:subClassOf sbeo:Impaired ;
                         rdfs:comment "Sensory impairment is when one of the senses such as sight, hearing, smell, touch, taste and spatial awareness, is no longer normal."^^xsd:string ;
                         rdfs:label "SensoryImpairment"^^xsd:string .


###  http://www.ia.urjc.es/ontologies/building/sbeo#SmokeSensor
sbeo:SmokeSensor rdf:type owl:Class ;
                   owl:equivalentClass saref:SmokeSensor ;
                   rdfs:subClassOf sbeo:Sensor ;
                   rdfs:comment "The smoke sensor is a type of sensors that detects the presence of smoke in a particular space where it has been installed."^^xsd:string ;
                   rdfs:label "SmokeSensor"^^xsd:string .


###  http://www.ia.urjc.es/ontologies/building/sbeo#SpaceCharacteristic
sbeo:SpaceCharacteristic rdf:type owl:Class ;
                           rdfs:comment "SpaceCharacteristic class defines important features of each space that are required to take various decisions during an evacuation process."^^xsd:string ;
                           rdfs:label "SpaceCharacteristic"^^xsd:string .


###  http://www.ia.urjc.es/ontologies/building/sbeo#Stampeding
sbeo:Stampeding rdf:type owl:Class ;
                  rdfs:subClassOf sbeo:Panic ;
                  rdfs:comment "A sudden and uncontrollable run by the group of people caused by panic."^^xsd:string ;
                  rdfs:label "Stampeding"^^xsd:string .


###  http://www.ia.urjc.es/ontologies/building/sbeo#Successful
sbeo:Successful rdf:type owl:Class ;
                  rdfs:subClassOf sbeo:EvacuationStatus ;
                  rdfs:comment "It represents that the person has successfully evacuated the building."^^xsd:string ;
                  rdfs:label "Successful"^^xsd:string .


###  http://www.ia.urjc.es/ontologies/building/sbeo#TemperatureSensor
sbeo:TemperatureSensor rdf:type owl:Class ;
                         owl:equivalentClass saref:TemperatureSensor ;
                         rdfs:subClassOf sbeo:Sensor ;
                         rdfs:comment "The temperature sensor is a type of sensors that detects the ambient temperature of a space where it has been installed."^^xsd:string ;
                         rdfs:label "TemperatureSensor"^^xsd:string .


###  http://www.ia.urjc.es/ontologies/building/sbeo#TerroristAttack
sbeo:TerroristAttack rdf:type owl:Class ;
                       rdfs:subClassOf sbeo:Incident ;
                       rdfs:comment "A surprise event involving the deliberate use of violence against the occupants of the buildings."^^xsd:string ;
                       rdfs:label "TerroristAttack"^^xsd:string .


###  http://www.ia.urjc.es/ontologies/building/sbeo#Unavailable
sbeo:Unavailable rdf:type owl:Class ;
                   rdfs:subClassOf sbeo:SpaceCharacteristic ;
                   rdfs:comment "This is used to specify the availability of a parituclar space, route, etc. If its unavailable, it means it is not accessible to any sbeo:Person."^^xsd:string ;
                   rdfs:label "Unavailable"^^xsd:string .


###  http://www.ia.urjc.es/ontologies/building/sbeo#Visitor
sbeo:Visitor rdf:type owl:Class ;
               rdfs:subClassOf sbeo:PedestrianCharacteristic .


###  http://www.ia.urjc.es/ontologies/building/sbeo#Visual
sbeo:Visual rdf:type owl:Class ;
              rdfs:subClassOf sbeo:SensoryImpairment ;
              rdfs:comment "It is a partial or total unability to see. It is also known as visual loss. Here, we considered a person having visual impairment who as severe low vision; 20/200 to 20/400 or higher."^^xsd:string ;
              rdfs:label "Visual"^^xsd:string .


###  http://www.ia.urjc.es/ontologies/building/sbeo#WaitingZone
sbeo:WaitingZone rdf:type owl:Class ;
                   rdfs:subClassOf sbeo:SafeZone ;
                   rdfs:comment "A space where people can wait to picked up either by their family members or  acquaintances or emergency rescue teams, during any incident. It is always considered as safe."^^xsd:string ;
                   rdfs:label "WaitingZone"^^xsd:string .


###  http://www.ia.urjc.es/ontologies/building/sbeo#Wheelchair
sbeo:Wheelchair rdf:type owl:Class ;
                  rdfs:subClassOf sbeo:PhysicalImpairment ;
                  rdfs:comment "It is a mobility device that is used by a person having any kind of tempoary or permanent physical impairment."^^xsd:string ;
                  rdfs:label "Wheelchair"^^xsd:string .

###  Generated by the OWL API (version 4.5.9.2019-02-01T07:24:44Z) https://github.com/owlcs/owlapi
