@prefix : <http://www.ia.urjc.es/ontologies/building/sbevac#> .
@prefix ns: <http://www.w3.org/2003/06/sw-vocab-status/ns#> .
@prefix owl: <http://www.w3.org/2002/07/owl#> .
@prefix rdf: <http://www.w3.org/1999/02/22-rdf-syntax-ns#> .
@prefix xml: <http://www.w3.org/XML/1998/namespace> .
@prefix xsd: <http://www.w3.org/2001/XMLSchema#> .
@prefix foaf: <http://xmlns.com/foaf/0.1/> .
@prefix obda: <https://w3id.org/obda/vocabulary#> .
@prefix rdfs: <http://www.w3.org/2000/01/rdf-schema#> .
@prefix seas: <https://w3id.org/seas/> .
@prefix vann: <http://purl.org/vocab/vann/> .
@prefix saref: <https://w3id.org/saref#> .
@prefix terms: <http://purl.org/dc/terms/> .
@prefix sbevac: <http://www.ia.urjc.es/ontologies/building/sbevac#> .
@prefix dcterms: <http://purl.org/dc/terms/> .
@prefix fiemser: <http://sites.google.com/site/smartappliancesproject/ontologies/fiemser#> .
@base <http://www.ia.urjc.es/ontologies/building/sbevac> .

<http://www.ia.urjc.es/ontologies/building/sbevac> rdf:type owl:Ontology ;
                                                    owl:versionIRI <http://www.ia.urjc.es/ontologies/building/sbevac/1.6> ;
                                                    owl:imports seas:BuildingOntology-1.0 ;
                                                    dcterms:creator "Qasim Khalid"@en ;
                                                    dcterms:description "The Smart Buildings Evacuation (SBEVAC) ontology is proposed to acquire knowledge of emergency evacuation (or egress) and to provide safe evacuation paths to the occupants of buildings during hazardous circumstances in a building. The goal of this ontology is not only to provide safe paths to the people, but also the paths will be feasible for people with respect to their physical characteristics and preferences. In this regard, we propose a knowledge base system for emergency evacuation in which we use the concept of a smart building. First, we define the concepts that are necessary to develop the proposed systems. Second, we develop the hierarchy to use these concepts. Third, we define the properties and characteristics of these concepts. Fourth, we introduce role restrictions, and at last, we introduce instances for particular scenarios to validate our foundation knowledge base. We use three different concepts in our ontology and integrate them with respect to our requirements. The first concept is knowledge about the building geometry, the second concept is the knowledge about the momentary situation of the building, and the third concept is the knowledge about the occupants of the building. We reuse seas:BuildingOntology to get geometry of the buildings. Also, it may limit the overlap with the following existing specialized ontologies such as FIEMSER ontology, gbXML ontology and ifcOWL ontology."@en ;
                                                    dcterms:title "SBEVAC: Smart Building Evacuation Ontology"@en ;
                                                    owl:versionInfo "1.6"@en .

#################################################################
#    Annotation properties
#################################################################

###  http://www.w3.org/2002/07/owl#sameAs
owl:sameAs rdf:type owl:AnnotationProperty .


#################################################################
#    Object Properties
#################################################################

###  http://www.ia.urjc.es/ontologies/building/sbevac#accompanying
sbevac:accompanying rdf:type owl:ObjectProperty ,
                             owl:SymmetricProperty ,
                             owl:TransitiveProperty ;
                    rdfs:domain sbevac:Person ;
                    rdfs:range sbevac:Person ;
                    rdfs:comment "This property is used to mention how who is accompanying who."@en ;
                    rdfs:label "accompanying"@en .


###  http://www.ia.urjc.es/ontologies/building/sbevac#acquaintanceOf
sbevac:acquaintanceOf rdf:type owl:ObjectProperty ,
                               owl:SymmetricProperty ;
                      rdfs:domain sbevac:Person ;
                      rdfs:range sbevac:Person ;
                      rdfs:comment "This property is used to represent any friend or acquaintace tie among occupants."@en ;
                      rdfs:label "acquaintanceOf"@en .


###  http://www.ia.urjc.es/ontologies/building/sbevac#adjacentTo
sbevac:adjacentTo rdf:type owl:ObjectProperty ,
                           owl:SymmetricProperty ;
                  rdfs:domain seas:Zone ;
                  rdfs:range seas:Zone ;
                  rdfs:comment "This property is used to mention the spaces that are adjacent to a specific space by a wall. This property is helpful for security purposes, for example, in case of any emergency situation when the seas:BuildingSpaceConnection, i.e. door, windows, are not accessible."@en ;
                  rdfs:label "adjacentTo"@en .


###  http://www.ia.urjc.es/ontologies/building/sbevac#assignedRoute
sbevac:assignedRoute rdf:type owl:ObjectProperty ;
                     rdfs:subPropertyOf owl:topObjectProperty ;
                     rdfs:domain sbevac:Person ;
                     rdfs:range sbevac:Route ;
                     rdfs:comment "This property is used to represent a route (rdf:list of connected spaces) that is assigned to person for safe evacuation." ;
                     rdfs:label "assignedRoute" .


###  http://www.ia.urjc.es/ontologies/building/sbevac#connectedTo
sbevac:connectedTo rdf:type owl:ObjectProperty ,
                            owl:SymmetricProperty ;
                   rdfs:domain seas:BuildingSpace ,
                               seas:BuildingSpaceConnection ;
                   rdfs:range seas:BuildingSpace ,
                              seas:BuildingSpaceConnection ;
                   rdfs:comment "This property is used to mention the connectivity of any seas:BuildingSpaceConnection or seas:BuildingSpace with each other."@en ;
                   rdfs:label "conectedTo"@en ;
                   owl:sameAs "seas:connectedTo" .


###  http://www.ia.urjc.es/ontologies/building/sbevac#dependentOn
sbevac:dependentOn rdf:type owl:ObjectProperty ;
                   owl:inverseOf sbevac:responsibleTo ;
                   rdf:type owl:TransitiveProperty ;
                   rdfs:domain sbevac:Person ;
                   rdfs:range sbevac:Person ;
                   rdfs:comment "This property is used to mention the dependency of a particular person on his/her responsible person"@en ;
                   rdfs:label "dependentOn"@en .


###  http://www.ia.urjc.es/ontologies/building/sbevac#distanceOf
sbevac:distanceOf rdf:type owl:ObjectProperty ,
                           owl:SymmetricProperty ;
                  rdfs:domain sbevac:Distance ;
                  rdfs:range seas:Zone ,
                             seas:ZoneConnection ;
                  rdfs:comment "This property is used to represent the distance between any two connected seas:BuildingSpaceConnection or seas:BuildingSpace."@en ;
                  rdfs:label "distanceOf"@en .


###  http://www.ia.urjc.es/ontologies/building/sbevac#endsIn
sbevac:endsIn rdf:type owl:ObjectProperty ;
              owl:inverseOf sbevac:startsFrom ;
              rdfs:domain sbevac:Route ;
              rdfs:range seas:BuildingSpace ,
                         seas:BuildingSpaceConnection ;
              rdfs:comment "This property is used to express the last space where the route ends. Generally, these are sbevac:Exit."@en ;
              rdfs:label "endsIn"@en .


###  http://www.ia.urjc.es/ontologies/building/sbevac#hasPath
sbevac:hasPath rdf:type owl:ObjectProperty ;
               rdfs:domain seas:BuildingSpace ,
                           seas:BuildingSpaceConnection ;
               rdfs:range seas:BuildingSpace ,
                          seas:BuildingSpaceConnection ;
               rdfs:comment "This property is used to express the set of connected spaces that makes a route."@en ;
               rdfs:label "hasPath"@en .


###  http://www.ia.urjc.es/ontologies/building/sbevac#installedIn
sbevac:installedIn rdf:type owl:ObjectProperty ,
                            owl:TransitiveProperty ;
                   rdfs:domain sbevac:Device ,
                               seas:BuildingSpace ,
                               seas:BuildingSpaceConnection ;
                   rdfs:range seas:BuildingSpace ,
                              seas:BuildingSpaceConnection ;
                   rdfs:comment "This property is used to mention any device, system, or instrument, installed in a seas:BuildingSpace."@en ;
                   rdfs:label "installedIn"@en .


###  http://www.ia.urjc.es/ontologies/building/sbevac#locatedIn
sbevac:locatedIn rdf:type owl:ObjectProperty ;
                 rdfs:subPropertyOf owl:topObjectProperty ;
                 rdf:type owl:TransitiveProperty ;
                 rdfs:domain sbevac:Incident ,
                             sbevac:Person ,
                             seas:Zone ,
                             seas:ZoneConnection ;
                 rdfs:range seas:BuildingSpaceConnection ,
                            seas:Zone ;
                 rdfs:comment "This property is used to mention the existence of anything in a particular seas:BuildingSpace, such as person, or stairs, doors, etc."@en ;
                 rdfs:label "locatedIn"@en .


###  http://www.ia.urjc.es/ontologies/building/sbevac#notAccessibleTo
sbevac:notAccessibleTo rdf:type owl:ObjectProperty ;
                       rdfs:domain seas:Zone ,
                                   seas:ZoneConnection ;
                       rdfs:range sbevac:Person ;
                       rdfs:comment "This property is used to prohibit the access of any specific person to a specific seas:BuildingSpace."@en ;
                       rdfs:label "notAccessibleTo"@en .


###  http://www.ia.urjc.es/ontologies/building/sbevac#responsibleTo
sbevac:responsibleTo rdf:type owl:ObjectProperty ;
                     rdfs:domain sbevac:Person ;
                     rdfs:range sbevac:Person ;
                     rdfs:comment "This property is used to mention the responsibility for a particular person to his/her dependent persons."@en ;
                     rdfs:label "responsibleTo"@en .


###  http://www.ia.urjc.es/ontologies/building/sbevac#startsFrom
sbevac:startsFrom rdf:type owl:ObjectProperty ;
                  rdfs:domain sbevac:Route ;
                  rdfs:range seas:Zone ,
                             seas:ZoneConnection ;
                  rdfs:comment "This property is used to express the last space where any route starts."@en ;
                  rdfs:label "startsFrom"@en .


###  https://w3id.org/seas/connectedTo
seas:connectedTo rdf:type owl:ObjectProperty .


#################################################################
#    Data properties
#################################################################

###  http://www.ia.urjc.es/ontologies/building/sbevac#accommodationCapacity
sbevac:accommodationCapacity rdf:type owl:DatatypeProperty ;
                             rdfs:domain seas:Zone ,
                                         seas:ZoneConnection ;
                             rdfs:range xsd:integer ;
                             rdfs:comment "This property is used to represent the accommodating capacity (in terms of persons) of a particular space."@en ;
                             rdfs:label "accommodationCapacity"@en .


###  http://www.ia.urjc.es/ontologies/building/sbevac#age
sbevac:age rdf:type owl:DatatypeProperty ;
           rdfs:comment "The age of the person."@en ;
           rdfs:label "age"@en ;
           owl:sameAs "foaf:age"@en .


###  http://www.ia.urjc.es/ontologies/building/sbevac#atTime
sbevac:atTime rdf:type owl:DatatypeProperty ;
              rdfs:domain sbevac:EvacuationStatus ,
                          sbevac:Incident ,
                          sbevac:Person ,
                          sbevac:Sensor ;
              rdfs:range xsd:long ;
              rdfs:comment "This property is used to attach a timestamp with any particular event."@en ;
              rdfs:label "atTime"@en .


###  http://www.ia.urjc.es/ontologies/building/sbevac#currentOccupancy
sbevac:currentOccupancy rdf:type owl:DatatypeProperty ;
                        rdfs:domain seas:Zone ,
                                    seas:ZoneConnection ;
                        rdfs:range xsd:integer ;
                        rdfs:comment "This property is used to represent the current occupancy(in terms of persons) of a particular space."@en ;
                        rdfs:label "currentOccupancy"@en .


###  http://www.ia.urjc.es/ontologies/building/sbevac#familiarityWithBuilding
sbevac:familiarityWithBuilding rdf:type owl:DatatypeProperty ;
                               rdfs:domain sbevac:Person ;
                               rdfs:range xsd:boolean ;
                               rdfs:comment "This property is used to represent the familiarity of person with the building geometry."@en ;
                               rdfs:label "familiarityWithBuilding"@en .


###  http://www.ia.urjc.es/ontologies/building/sbevac#familyID
sbevac:familyID rdf:type owl:DatatypeProperty ;
                rdfs:domain sbevac:Person ;
                rdfs:range xsd:integer ;
                rdfs:comment "This property is used to represent an identity number(ID) of each family. All the members of a family have common ID."@en ;
                rdfs:label "familyID"@en .


###  http://www.ia.urjc.es/ontologies/building/sbevac#firstName
sbevac:firstName rdf:type owl:DatatypeProperty ;
                 rdfs:subPropertyOf owl:topDataProperty ;
                 rdfs:comment "The first name of the person."@en ;
                 rdfs:label "firstName"@en ;
                 owl:sameAs "foaf:firstName"@en .


###  http://www.ia.urjc.es/ontologies/building/sbevac#fitnessLevel
sbevac:fitnessLevel rdf:type owl:DatatypeProperty ;
                    rdfs:domain sbevac:Person ;
                    rdfs:range xsd:integer ;
                    rdfs:comment "This property is used to represent the fitness level of a person. For example, there are 5 levels. Upper three levels are appropriate and considered as safe whereas the below two levels are considered as dangerous and a particular person needs assistance. The person is considered as sbevac:Injured, if the levels are changed from upper three to lower two."@en ;
                    rdfs:label "fitnessLevel"@en .


###  http://www.ia.urjc.es/ontologies/building/sbevac#groupID
sbevac:groupID rdf:type owl:DatatypeProperty ;
               rdfs:domain sbevac:Person ;
               rdfs:range xsd:integer ;
               rdfs:comment "This property is used to represent an identity number(ID) that is assigned to people who are evacuating together and having the same sbevac:assignedRoute."@en ;
               rdfs:label "groupID"@en .


###  http://www.ia.urjc.es/ontologies/building/sbevac#hasID
sbevac:hasID rdf:type owl:DatatypeProperty ;
             rdfs:domain sbevac:Person ;
             rdfs:range xsd:integer ;
             rdfs:comment "This property is used to represent an identification number, which is unique for every occupant of the building. It is different than group and family ID. This ID number is used to calculate all the functionalities for a specific person, e.g. location, characteristics, preferences, etc."@en ;
             rdfs:label "hasID"@en .


###  http://www.ia.urjc.es/ontologies/building/sbevac#hasLength
sbevac:hasLength rdf:type owl:DatatypeProperty ;
                 rdfs:domain sbevac:Route ;
                 rdfs:range xsd:integer ;
                 rdfs:comment "This property is used to represent a value between any two building space connections. This value can be expressed in terms of time, distance, etc."@en ;
                 rdfs:label "hasLength"@en .


###  http://www.ia.urjc.es/ontologies/building/sbevac#lastName
sbevac:lastName rdf:type owl:DatatypeProperty ;
                rdfs:subPropertyOf owl:topDataProperty ;
                rdfs:comment "The last name of the person."@en ;
                rdfs:label "lastName"@en ;
                owl:sameAs "foaf:lastName"@en .


###  http://www.ia.urjc.es/ontologies/building/sbevac#name
sbevac:name rdf:type owl:DatatypeProperty ;
            rdfs:label "The name of the person, place or a thing."@en ,
                       "name"@en ;
            owl:sameAs "foaf:name"@en .


###  http://www.ia.urjc.es/ontologies/building/sbevac#needsSupervision
sbevac:needsSupervision rdf:type owl:DatatypeProperty ;
                        rdfs:domain sbevac:Person ;
                        rdfs:range xsd:boolean ;
                        rdfs:comment "This property is used to mention either a person needs a supervision or not."@en ;
                        rdfs:label "needsSupervision"@en .


#################################################################
#    Classes
#################################################################

###  http://www.ia.urjc.es/ontologies/building/sbevac#ActiveFireProtection
sbevac:ActiveFireProtection rdf:type owl:Class ;
                            rdfs:subClassOf sbevac:FireProtection ;
                            rdfs:comment "ActiveFireProtection"@en ,
                                         "It is an integral part of the fire protection used as a first response to minimize the spread of fire and related effects."@en .


###  http://www.ia.urjc.es/ontologies/building/sbevac#AssemblyPoint
sbevac:AssemblyPoint rdf:type owl:Class ;
                     rdfs:subClassOf sbevac:SafeZone ;
                     rdfs:comment "a place where people in an office, etc. should go if there is an emergency, for example, a fire (Cambridge English Dictionary) ."@en ;
                     rdfs:label "AssemblyPoint"@en .


###  http://www.ia.urjc.es/ontologies/building/sbevac#Available
sbevac:Available rdf:type owl:Class ;
                 owl:equivalentClass sbevac:SafeZone ;
                 rdfs:subClassOf sbevac:SpaceCharacteristic ;
                 owl:disjointWith sbevac:Unavailable ;
                 rdfs:comment "This is used to specify the availability of a parituclar space, route, etc. If its available, it means it can be accessible to sbevac:Person subject to the characteristics of that person."@en ;
                 rdfs:label "Available"@en .


###  http://www.ia.urjc.es/ontologies/building/sbevac#ChemicalSpill
sbevac:ChemicalSpill rdf:type owl:Class ;
                     rdfs:subClassOf sbevac:Incident ;
                     rdfs:comment "A hazardous event that happens due to the spillage or leakge of any toxic chemical in the building."@en ;
                     rdfs:label "ChemicalSpill"@en .


###  http://www.ia.urjc.es/ontologies/building/sbevac#Congestion
sbevac:Congestion rdf:type owl:Class ;
                  rdfs:subClassOf sbevac:Incident ;
                  rdfs:comment "An event that happens at bottlenecks when the flow of people increases than a provided limit due to herding (and similar phenomena of human behaviour), during an emergency evacuation process. As a result, overall escape time is increased."@en ;
                  rdfs:label "Congestion"@en .


###  http://www.ia.urjc.es/ontologies/building/sbevac#DayCare
sbevac:DayCare rdf:type owl:Class ;
               rdfs:subClassOf seas:Room ;
               rdfs:comment "A space for childcare supervised by a nanny while parents are at work."@en ;
               rdfs:label "DayCare"@en .


###  http://www.ia.urjc.es/ontologies/building/sbevac#Dependent
sbevac:Dependent rdf:type owl:Class ;
                 rdfs:subClassOf sbevac:PedestrianCharacteristic ;
                 owl:disjointWith sbevac:Responsible ;
                 rdfs:comment "It represents the dependency of a person on other persons in case of any emergency condition."@en ;
                 rdfs:label "Dependent"@en .


###  http://www.ia.urjc.es/ontologies/building/sbevac#Device
sbevac:Device rdf:type owl:Class ;
              rdfs:comment "A thing made or adapted for a particular purpose, especially a piece of mechanical or electronic equipment (Oxford Dictionary of English)."@en ;
              rdfs:label "Device"@en .


###  http://www.ia.urjc.es/ontologies/building/sbevac#Distance
sbevac:Distance rdf:type owl:Class ;
                rdfs:subClassOf sbevac:SpaceCharacteristic ;
                rdfs:comment "Distance class is mainly used to mention the distance between two spaces(either connected or not). As the building is represented as a graph having nodes and egdes, where as edges represents the connection between two nodes, therefore, the weight of the edge is considered as the Distance. Later on, the Distance is used to calculate the evaucation routes."@en ;
                rdfs:label "Distance"@en .


###  http://www.ia.urjc.es/ontologies/building/sbevac#Earthquake
sbevac:Earthquake rdf:type owl:Class ;
                  rdfs:subClassOf sbevac:Incident ;
                  rdfs:comment "A sudden violent shaking of the ground, typically causing great destruction, as a result of movements within the earth's crust or volcanic action(Oxford Dictionary). It may cause a sudden panic among the occupants of the building."@en ;
                  rdfs:label "Earthquake"@en .


###  http://www.ia.urjc.es/ontologies/building/sbevac#EmergencyExit
sbevac:EmergencyExit rdf:type owl:Class ;
                     rdfs:subClassOf sbevac:Exit ;
                     rdfs:comment "Emerency exit is only used in case of any emergency conditions such fire, etc."@en ;
                     rdfs:label "EmergencyExit"@en .


###  http://www.ia.urjc.es/ontologies/building/sbevac#Entrance
sbevac:Entrance rdf:type owl:Class ;
                rdfs:subClassOf sbevac:SpaceCharacteristic ;
                rdfs:comment "Entrance represents a space or a door that is used to enter into a building. Normally, it is also used as an exit."@en ;
                rdfs:label "Entrance"@en .


###  http://www.ia.urjc.es/ontologies/building/sbevac#EvacuationStatus
sbevac:EvacuationStatus rdf:type owl:Class ;
                        rdfs:comment "The status of an evacuation process for each person."@en ;
                        rdfs:label "EvacuationStatus"@en .


###  http://www.ia.urjc.es/ontologies/building/sbevac#Exit
sbevac:Exit rdf:type owl:Class ;
            rdfs:subClassOf sbevac:SpaceCharacteristic ;
            rdfs:comment "Exit represents a space or a door that is used to exit the building. Generally, an exit is as same as an entrance."@en ;
            rdfs:label "Exit"@en .


###  http://www.ia.urjc.es/ontologies/building/sbevac#Family
sbevac:Family rdf:type owl:Class ;
              rdfs:subClassOf sbevac:PedestrianCharacteristic ;
              rdfs:comment "A group of persons having family ties between them."@en ;
              rdfs:label "Family"@en .


###  http://www.ia.urjc.es/ontologies/building/sbevac#Fire
sbevac:Fire rdf:type owl:Class ;
            rdfs:subClassOf sbevac:Incident ;
            rdfs:comment "An event that may burn different parts of the building and hazourdous for both the people and the building."@en ;
            rdfs:label "Fire"@en .


###  http://www.ia.urjc.es/ontologies/building/sbevac#FireDoor
sbevac:FireDoor rdf:type owl:Class ;
                rdfs:subClassOf sbevac:PassiveFireProtection ;
                rdfs:comment "A type of door used to minimize the spread of fire and related effects by isolating two connected spaces or sections in the building."@en ;
                rdfs:label "FireDoor"@en .


###  http://www.ia.urjc.es/ontologies/building/sbevac#FireExtinguisher
sbevac:FireExtinguisher rdf:type owl:Class ;
                        rdfs:subClassOf sbevac:ActiveFireProtection ;
                        rdfs:comment "An active fire protection instrument used by persons to blow out small scale fire."@en ;
                        rdfs:label "FireExtinguisher"@en .


###  http://www.ia.urjc.es/ontologies/building/sbevac#FireProtection
sbevac:FireProtection rdf:type owl:Class ;
                      rdfs:subClassOf sbevac:IncidentProtection ;
                      rdfs:comment "It is a practice to minimize the effects of potentially danger fires."@en ;
                      rdfs:label "FireProtection"@en .


###  http://www.ia.urjc.es/ontologies/building/sbevac#Hearing
sbevac:Hearing rdf:type owl:Class ;
               rdfs:subClassOf sbevac:SensoryImpairment ;
               rdfs:comment "It is a partial or total unability to hear. It is also known as Hearing loss."@en ;
               rdfs:label "Hearing"@en .


###  http://www.ia.urjc.es/ontologies/building/sbevac#Impaired
sbevac:Impaired rdf:type owl:Class ;
                owl:equivalentClass sbevac:Injured ;
                rdfs:subClassOf sbevac:PedestrianCharacteristic ;
                owl:disjointWith sbevac:Normal ;
                rdfs:comment "The state or fact of being impaired, especially in a specified faculty(Oxford Distionary of Language)."@en ;
                rdfs:label "Impaired"@en .


###  http://www.ia.urjc.es/ontologies/building/sbevac#InProgress
sbevac:InProgress rdf:type owl:Class ;
                  rdfs:subClassOf sbevac:NotSuccessful ;
                  rdfs:comment "It represents that the person is following the provided route and the evacuation process is in progress."@en ;
                  rdfs:label "InProgress"@en .


###  http://www.ia.urjc.es/ontologies/building/sbevac#Incident
sbevac:Incident rdf:type owl:Class ;
                rdfs:comment "An event or occurance that can be dangerous for the occupants of the building."@en ;
                rdfs:label "Incident"@en .


###  http://www.ia.urjc.es/ontologies/building/sbevac#IncidentProtection
sbevac:IncidentProtection rdf:type owl:Class ;
                          rdfs:subClassOf sbevac:Device ;
                          rdfs:comment "It is a practice to avoid and minimize the effects of potentially danger events for the occupants of the building as well as for the structure of building itself."@en ;
                          rdfs:label "IncidentProtection"@en .


###  http://www.ia.urjc.es/ontologies/building/sbevac#Injured
sbevac:Injured rdf:type owl:Class ;
               rdfs:subClassOf sbevac:PedestrianCharacteristic ;
               rdfs:comment "It represents an injury to a person during an evacuation process."@en ;
               rdfs:label "Injured"@en .


###  http://www.ia.urjc.es/ontologies/building/sbevac#KidsArea
sbevac:KidsArea rdf:type owl:Class ;
                rdfs:subClassOf seas:Room ;
                rdfs:comment "A space where children can play during the specific time while parents are either busy at work or doing different things such as shopping, seeing a doctor, etc. Normally, it is not supervised by anyone."@en ;
                rdfs:label "KidsArea"@en .


###  http://www.ia.urjc.es/ontologies/building/sbevac#LocationSensor
sbevac:LocationSensor rdf:type owl:Class ;
                      rdfs:subClassOf sbevac:Sensor ;
                      rdfs:comment "The location sensor is a part of indoor positioning system to detect the location of each person within the building."@en ;
                      rdfs:label "LocationSensor"@en .


###  http://www.ia.urjc.es/ontologies/building/sbevac#LowStamina
sbevac:LowStamina rdf:type owl:Class ;
                  rdfs:subClassOf sbevac:PhysicalImpairment ;
                  rdfs:comment "It is the unability to sustain physical or mental activity to a normal level."@en ;
                  rdfs:label "LowStamina"@en .


###  http://www.ia.urjc.es/ontologies/building/sbevac#Motorised
sbevac:Motorised rdf:type owl:Class ;
                 rdfs:subClassOf sbevac:Wheelchair ;
                 rdfs:comment "It is a kind of wheelchair that has either a mechanical engine or an electric battery. It has more speed than a traditional wheelchair."@en ;
                 rdfs:label "Motorised"@en .


###  http://www.ia.urjc.es/ontologies/building/sbevac#Non-Motorised
sbevac:Non-Motorised rdf:type owl:Class ;
                     rdfs:subClassOf sbevac:Wheelchair ;
                     rdfs:comment "A traditional wheelchair that is used by hands. It has significantly lower speed than motorised wheelchairs."@en ;
                     rdfs:label "Non-Motorised"@en .


###  http://www.ia.urjc.es/ontologies/building/sbevac#Normal
sbevac:Normal rdf:type owl:Class ;
              rdfs:subClassOf sbevac:PedestrianCharacteristic ;
              rdfs:comment "Persons who are not having any impairment."@en ;
              rdfs:label "Normal"@en .


###  http://www.ia.urjc.es/ontologies/building/sbevac#NormalExit
sbevac:NormalExit rdf:type owl:Class ;
                  rdfs:subClassOf sbevac:Exit ;
                  rdfs:comment "Normal exit is used to exit a building. It can be a door or the whole space in the building that is always considered safe."@en ;
                  rdfs:label "NormalExit"@en .


###  http://www.ia.urjc.es/ontologies/building/sbevac#NotSuccessful
sbevac:NotSuccessful rdf:type owl:Class ;
                     rdfs:subClassOf sbevac:EvacuationStatus ;
                     rdfs:comment "It represents that the evacuation is not completed by a person yet."@en ;
                     rdfs:label "NotSuccessful"@en .


###  http://www.ia.urjc.es/ontologies/building/sbevac#Obstructed
sbevac:Obstructed rdf:type owl:Class ;
                  rdfs:subClassOf sbevac:NotSuccessful ;
                  rdfs:comment "It represents that the person is obstrcuted during an evacuation process and not continuing one's evcuation."@en ;
                  rdfs:label "Obstructed"@en .


###  http://www.ia.urjc.es/ontologies/building/sbevac#Panic
sbevac:Panic rdf:type owl:Class ;
             rdfs:subClassOf sbevac:Incident ;
             rdfs:comment "A  sudden uncontrollable fear or anxiety, often causing wildly unthinking behaviour (Oxford Dictionary of English)."@en ;
             rdfs:label "Panic"@en .


###  http://www.ia.urjc.es/ontologies/building/sbevac#PassiveFireProtection
sbevac:PassiveFireProtection rdf:type owl:Class ;
                             rdfs:subClassOf sbevac:FireProtection ;
                             rdfs:comment "It is an integral component installed in the building while construction to resist the fire."@en ;
                             rdfs:label "PassiveFireProtection"@en .


###  http://www.ia.urjc.es/ontologies/building/sbevac#PedestrianCharacteristic
sbevac:PedestrianCharacteristic rdf:type owl:Class ;
                                rdfs:comment "PedestrianCharacteristic class defines features for each person that are helps system to find an appropriate route."@en ;
                                rdfs:label "PedestrianCharacteristic"@en .


###  http://www.ia.urjc.es/ontologies/building/sbevac#Person
sbevac:Person rdf:type owl:Class ;
              rdfs:comment "It represents a single individual of any age and having any type of characteristics."@en ;
              rdfs:label "Person"@en ;
              owl:sameAs "http://xmlns.com/foaf/0.1/Person" .


###  http://www.ia.urjc.es/ontologies/building/sbevac#PhysicalImpairment
sbevac:PhysicalImpairment rdf:type owl:Class ;
                          rdfs:subClassOf sbevac:Impaired ;
                          rdfs:comment "A physical impairment is a condition in which any part of person's body is either  damaged or is not working properly."@en ;
                          rdfs:label "PhysicalImpairment"@en .


###  http://www.ia.urjc.es/ontologies/building/sbevac#Responsible
sbevac:Responsible rdf:type owl:Class ;
                   rdfs:subClassOf sbevac:PedestrianCharacteristic ;
                   rdfs:comment "This class represents either a person is reponsible to anyone or not. One may be reponsible to one/all of one's family members or any other person such as injured, impiared etc."@en ;
                   rdfs:label "Responsible"@en .


###  http://www.ia.urjc.es/ontologies/building/sbevac#Route
sbevac:Route rdf:type owl:Class ;
             rdfs:subClassOf sbevac:SpaceCharacteristic ;
             rdfs:comment "Route is a set of spaces connected to each other by a door that ultimately leads to any of the exits in the building. Technically, rdf:list is used to store it."@en ;
             rdfs:label "Route"@en .


###  http://www.ia.urjc.es/ontologies/building/sbevac#SafeZone
sbevac:SafeZone rdf:type owl:Class ;
                rdfs:subClassOf sbevac:SpaceCharacteristic ;
                rdfs:comment "A space that is considered safe during any type of incident in the building."@en ;
                rdfs:label "SafeZone"@en .


###  http://www.ia.urjc.es/ontologies/building/sbevac#Sensor
sbevac:Sensor rdf:type owl:Class ;
              rdfs:subClassOf sbevac:Device ;
              rdfs:comment "A sensor is device that detects or measures a physical property and records, indicates, or otherwise responds to it (Oxford Dictionary of English)."@en ;
              rdfs:label "Sensor"@en ;
              owl:sameAs "https://w3id.org/saref#Sensor" .


###  http://www.ia.urjc.es/ontologies/building/sbevac#SensoryImpairment
sbevac:SensoryImpairment rdf:type owl:Class ;
                         rdfs:subClassOf sbevac:Impaired ;
                         rdfs:comment "Sensory impairment is when one of the senses such as sight, hearing, smell, touch, taste and spatial awareness, is no longer normal."@en ;
                         rdfs:label "SensoryImpairment"@en .


###  http://www.ia.urjc.es/ontologies/building/sbevac#SmokeSensor
sbevac:SmokeSensor rdf:type owl:Class ;
                   rdfs:subClassOf sbevac:Sensor ;
                   rdfs:comment "The smoke sensor is a type of sensors that detects the presence of smoke in a particular space where it has been installed."@en ;
                   rdfs:label "SmokeSensor"@en ;
                   owl:sameAs "https://w3id.org/saref#SmokeSensor" .


###  http://www.ia.urjc.es/ontologies/building/sbevac#SpaceCharacteristic
sbevac:SpaceCharacteristic rdf:type owl:Class ;
                           rdfs:comment "SpaceCharacteristic class defines important features of each space that are required to take various decisions during an evacuation process."@en ;
                           rdfs:label "SpaceCharacteristic"@en .


###  http://www.ia.urjc.es/ontologies/building/sbevac#Stampeding
sbevac:Stampeding rdf:type owl:Class ;
                  rdfs:subClassOf sbevac:Panic ;
                  rdfs:comment "A sudden and uncontrollable run by the group of people caused by panic."@en ;
                  rdfs:label "Stampeding"@en .


###  http://www.ia.urjc.es/ontologies/building/sbevac#Successful
sbevac:Successful rdf:type owl:Class ;
                  rdfs:subClassOf sbevac:EvacuationStatus ;
                  rdfs:comment "It represents that the person has successfully evacuated the building."@en ;
                  rdfs:label "Successful"@en .


###  http://www.ia.urjc.es/ontologies/building/sbevac#TemperatureSensor
sbevac:TemperatureSensor rdf:type owl:Class ;
                         rdfs:subClassOf sbevac:Sensor ;
                         rdfs:comment "The temperature sensor is a type of sensors that detects the ambient temperature of a space where it has been installed."@en ;
                         rdfs:label "TemperatureSensor"@en ;
                         owl:sameAs "https://w3id.org/saref#TemperatureSensor" .


###  http://www.ia.urjc.es/ontologies/building/sbevac#TerroristAttack
sbevac:TerroristAttack rdf:type owl:Class ;
                       rdfs:subClassOf sbevac:Incident ;
                       rdfs:comment "A surprise event involving the deliberate use of violence against the occupants of the buildings."@en ;
                       rdfs:label "TerroristAttack"@en .


###  http://www.ia.urjc.es/ontologies/building/sbevac#Unavailable
sbevac:Unavailable rdf:type owl:Class ;
                   rdfs:subClassOf sbevac:SpaceCharacteristic ;
                   rdfs:comment "This is used to specify the availability of a parituclar space, route, etc. If its unavailable, it means it is not accessible to any sbevac:Person."@en ;
                   rdfs:label "Unavailable"@en .


###  http://www.ia.urjc.es/ontologies/building/sbevac#Visitor
sbevac:Visitor rdf:type owl:Class ;
               rdfs:subClassOf sbevac:PedestrianCharacteristic .


###  http://www.ia.urjc.es/ontologies/building/sbevac#Visual
sbevac:Visual rdf:type owl:Class ;
              rdfs:subClassOf sbevac:SensoryImpairment ;
              rdfs:comment "It is a partial or total unability to see. It is also known as visual loss. Here, we considered a person having visual impairment who as severe low vision; 20/200 to 20/400 or higher."@en ;
              rdfs:label "Visual"@en .


###  http://www.ia.urjc.es/ontologies/building/sbevac#WaitingZone
sbevac:WaitingZone rdf:type owl:Class ;
                   rdfs:subClassOf sbevac:SafeZone ;
                   rdfs:comment "A space where people can wait to picked up either by their family members or  acquaintances or emergency rescue teams, during any incident. It is always considered as safe."@en ;
                   rdfs:label "WaitingZone"@en .


###  http://www.ia.urjc.es/ontologies/building/sbevac#Wheelchair
sbevac:Wheelchair rdf:type owl:Class ;
                  rdfs:subClassOf sbevac:PhysicalImpairment ;
                  rdfs:comment "It is a mobility device that is used by a person having any kind of tempoary or permanent physical impairment."@en ;
                  rdfs:label "Wheelchair"@en .


###  https://w3id.org/seas/Room
seas:Room rdf:type owl:Class .


###  Generated by the OWL API (version 4.5.9.2019-02-01T07:24:44Z) https://github.com/owlcs/owlapi
